player.lean
@@ -62,22 +62,25 @@ def Angel.sup {pw pw₁ : ℕ} (a₁ : Angel pw₁) (a : Angel pw) : Prop :=
 def Angel.sub {pw₁ pw : ℕ} (a : Angel pw₁) (a₁ : Angel pw) : Prop :=
 a₁.sup a
 
-def Valid_move_T := Board → Type
+def Angel_prev_moves (pw : ℕ) (s : State) :=
+Π (s₁ : State), s₁.history.length < s.history.length →
+angel_has_valid_move pw s₁.board → Valid_angel_move pw s₁.board
 
-def Prev_moves (T : Valid_move_T) (s : State) :=
-Π (s₁ : State), s₁.history.length < s.history.length → T s₁.board
+def Devil_prev_moves (s : State) :=
+Π (s₁ : State), s₁.history.length < s.history.length →
+Valid_devil_move s₁.board
 
-def Angel.set_prev_moves {pw : ℕ} {s : State} (a : Angel pw)
-  (pm : Prev_moves (Valid_angel_move pw) s) : Angel pw :=
+def Angel.set_prev_moves {pw : ℕ} (a : Angel pw) (s : State)
+  (pm : Angel_prev_moves pw s) : Angel pw :=
 begin
-  refine ⟨λ s₁ h, _⟩,
-  apply dite (s₁.history.length < s.history.length); intro h₁,
-  { exact pm s₁ h₁ },
-  { exact a.f s₁ h },
+  refine ⟨λ s₁ h₁, _⟩,
+  apply dite (s₁.history.length < s.history.length); intro h₂,
+  { exact pm s₁ h₂ h₁ },
+  { exact a.f s₁ h₁ },
 end
 
-def Devil.set_prev_moves {s : State} (d : Devil)
-  (pm : Prev_moves Valid_devil_move s) : Devil :=
+def Devil.set_prev_moves (d : Devil) (s : State)
+  (pm : Devil_prev_moves s) : Devil :=
 begin
   refine ⟨λ s₁, _⟩,
   apply dite (s₁.history.length < s.history.length); intro h₁,
@@ -99,6 +102,32 @@ begin
   refine ⟨λ s₁, _⟩, apply dite (s₁ = s); intro h₁,
   { cases h₁, exact md },
   { exact d.f s₁ },
+end
+
+def Angel.prev_moves_id {pw : ℕ} (a : Angel pw) (s : State) : Angel pw :=
+a.set_prev_moves s (λ s₁ _ h, a.f s₁ h)
+
+def Devil.prev_moves_id (d : Devil) (s : State) : Devil :=
+d.set_prev_moves s (λ s₁ h, d.f s₁)
+
+def Angel.prev_moves_set {pw : ℕ} (a : Angel pw) (s : State)
+  (s₁ : State) (m : Valid_angel_move pw s₁.board)
+  (h : s₁.history.length < s.history.length) : Angel pw :=
+begin
+  apply a.set_prev_moves s, rintro s₂ h₁ h₂,
+  apply dite (s₂ = s₁); intro h₃,
+  { cases h₃, exact m },
+  { exact a.f s₂ h₂ },
+end
+
+def Devil.prev_moves_set (d : Devil) (s : State)
+  (s₁ : State) (m : Valid_devil_move s₁.board)
+  (h : s₁.history.length < s.history.length) : Devil :=
+begin
+  apply d.set_prev_moves s, rintro s₂ h₁,
+  apply dite (s₂ = s₁); intro h₂,
+  { cases h₂, exact m },
+  { exact d.f s₂ },
 end
 
 -----
@@ -127,4 +156,84 @@ begin
   split; intro h,
   { subst h, simp },
   { cases d₁ with f₁, cases d₂ with f₂, congr, ext, apply h },
+end
+
+lemma angel_prev_moves_id_eq {pw : ℕ} {a : Angel pw} {s : State} :
+  a.prev_moves_id s = a :=
+by { rw angels_eq_iff, rintro s₁ h, change dite _ _ _ = _, split_ifs; refl }
+
+lemma devil_prev_moves_id_eq {d : Devil} {s : State} :
+  d.prev_moves_id s = d :=
+by { rw devils_eq_iff, rintro s₁, change dite _ _ _ = _, split_ifs; refl }
+
+lemma angel_set_move_eq {pw : ℕ} {a : Angel pw}
+  {s : State} {m : Valid_angel_move pw s.board} {h} :
+  (a.set_move s m).f s h = m :=
+by { change dite _ _ _ = _, split_ifs with h₁; refl }
+
+lemma devil_set_move_eq {d : Devil}
+  {s : State} {m : Valid_devil_move s.board} :
+  (d.set_move s m).f s = m :=
+by { change dite _ _ _ = _, split_ifs with h₁; refl }
+
+lemma angel_set_move_self {pw : ℕ} {a : Angel pw}
+  {s : State} {h} : a.set_move s (a.f s h) = a :=
+begin
+  rw angels_eq_iff; intros, change dite _ _ _ = _, split_ifs with h₂,
+  { subst h₂ }, { refl },
+end
+
+lemma devil_set_move_self {d : Devil}
+  {s : State} : d.set_move s (d.f s) = d :=
+begin
+  rw devils_eq_iff; intros, change dite _ _ _ = _, split_ifs with h₂,
+  { subst h₂ }, { refl },
+end
+
+lemma angel_set_move_set_move_eq {pw : ℕ} {a : Angel pw} {s : State}
+  {m₁ m₂ : Valid_angel_move pw s.board} :
+  (a.set_move s m₁).set_move s m₂ = a.set_move s m₂ :=
+begin
+  rw angels_eq_iff, rintro s₁ h₁,
+  change dite _ _ _ = _, split_ifs with h₂,
+  { subst h₂, rw angel_set_move_eq },
+  { change dite _ _ _ = dite _ _ _, simp_rw dif_neg h₂ },
+end
+
+lemma devil_set_move_set_move_eq {d : Devil} {s : State}
+  {m₁ m₂ : Valid_devil_move s.board} :
+  (d.set_move s m₁).set_move s m₂ = d.set_move s m₂ :=
+begin
+  rw devils_eq_iff, rintro s₁,
+  change dite _ _ _ = _, split_ifs with h₂,
+  { subst h₂, rw devil_set_move_eq },
+  { change dite _ _ _ = dite _ _ _, simp_rw dif_neg h₂ },
+end
+
+lemma angel_prev_moves_set_eq {pw : ℕ} {a : Angel pw} {s s₁ : State}
+  {m : Valid_angel_move pw s₁.board} {h} :
+  a.prev_moves_set s s₁ m h = a.set_move s₁ m :=
+begin
+  rw angels_eq_iff, rintro s₂ h,
+  change dite _ _ _ = _, split_ifs with h₁,
+  { dsimp, split_ifs with h₂,
+    { subst h₂, simp [angel_set_move_eq] },
+    { change _ = dite _ _ _, rw dif_neg h₂ }},
+  { change _ = dite _ _ _, split_ifs with h₂,
+    { subst h₂, contradiction },
+    { refl }},
+end
+
+lemma devil_prev_moves_set_eq {d : Devil} {s s₁ : State}
+  {m : Valid_devil_move s₁.board} {h} :
+  d.prev_moves_set s s₁ m h = d.set_move s₁ m :=
+begin
+  rw devils_eq_iff, rintro s₂,
+  change dite _ _ _ = _, split_ifs with h₁,
+  { dsimp, split_ifs with h₂,
+    { subst h₂, simp [devil_set_move_eq] },
+    { change _ = dite _ _ _, rw dif_neg h₂ }},
+  { change _ = dite _ _ _, split_ifs with h₂,
+    { subst h₂, contradiction },
+    { refl }},
 end
